Phi_Semantics/PhSem_BC_Storage.thy
@@ -1,0 +1,10 @@
+theory PhSem_BC_Storage
+  imports Phi_System.Resource_Template
+begin
+
+section \<open>Semantics\<close>
+
+
+
+
+end
